theories/crypto/rom/PROM.ec
@@ -352,9 +352,9 @@ abstract theory GenEager.
   equiv I_f_eqex x1 mx1 mx2: RRO.I.f ~ RRO.I.f :
          ={x}
       /\ x1 <> x{1}
-      /\ eq_except FRO.m{1} FRO.m{2} (fset1 x1)
+      /\ eq_except FRO.m{1} FRO.m{2} (pred1 x1)
       /\ FRO.m{1}.[x1] = mx1 /\ FRO.m{2}.[x1] = mx2
-    ==>    eq_except FRO.m{1} FRO.m{2} (fset1 x1)
+    ==>    eq_except FRO.m{1} FRO.m{2} (pred1 x1)
         /\ FRO.m{1}.[x1] = mx1
         /\ FRO.m{2}.[x1] = mx2.
   proof.
@@ -396,7 +396,7 @@ abstract theory GenEager.
       (={x,FRO.m} /\ mem (dom FRO.m{1}) x{1} /\ (oget FRO.m{1}.[x{1}]).`2 = Unknown ==>
        ={x,FRO.m})
       (={x,FRO.m} /\ mem (dom FRO.m{1}) x{1} /\ (oget FRO.m{1}.[x{1}]).`2 = Unknown==>
-       ={x} /\ eq_except FRO.m{1} FRO.m{2} (fset1 x{1}) /\
+       ={x} /\ eq_except FRO.m{1} FRO.m{2} (pred1 x{1}) /\
        FRO.m{1}.[x{2}] = Some (result{2},Unknown) /\
        FRO.m{2}.[x{2}] = Some (result{2},Known)).
     + by move=> ? &mr [#] -> -> ? ?; exists FRO.m{mr}, x{mr}=> /#.
@@ -408,7 +408,7 @@ abstract theory GenEager.
       skip=> &1 &2 [[->> ->>]] [Hdom Hm]; split=>//=.
       by apply /perm_eq_sym/perm_to_rem/dom_restr; rewrite /in_dom_with Hdom Hm.
     inline Iter(RRO.I).iter_1s RRO.I.f RRO.resample.
-    seq 5 3 : (={x} /\ eq_except FRO.m{1} FRO.m{2} (fset1 x{1}) /\
+    seq 5 3 : (={x} /\ eq_except FRO.m{1} FRO.m{2} (pred1 x{1}) /\
                (l = elems (dom (restr Unknown FRO.m) `\` fset1 x)){1} /\
                FRO.m{1}.[x{2}] = Some (result{2}, Unknown) /\
                FRO.m{2}.[x{2}] = Some (result{2}, Known)).
@@ -417,12 +417,12 @@ abstract theory GenEager.
     exists* x{1}, FRO.m{1}.[x{2}], FRO.m{2}.[x{2}]; elim*=>x1 mx1 mx2.
     call (iter_inv RRO.I
            (fun z=> x1 <> z) 
-           (fun o1 o2 => eq_except o1 o2 (fset1 x1) /\ o1.[x1]= mx1 /\ o2.[x1]=mx2)
+           (fun o1 o2 => eq_except o1 o2 (pred1 x1) /\ o1.[x1]= mx1 /\ o2.[x1]=mx2)
            (I_f_eqex x1 mx1 mx2))=> /=.
     + auto=> ? &mr [#] 4-> ^H -> -> ^H1 -> ^H2 -> /=; split.
       + congr; rewrite fsetP=> z; rewrite !inE !dom_restr /in_dom_with !in_dom.
         case: (z = x{mr})=> /= [->|]; 1:by rewrite H2 /= oget_some.
-        by move: H=> /eq_exceptP h; move: (h z); rewrite !inE=> {h} h /h ->.
+        by move: H=> /eq_exceptP h; move: (h z)=> {h} h /h ->.
     by move=> x; rewrite -memE in_fsetD1 eq_sym.
   swap{1}-1; seq  1  1: (={r,x,FRO.m} /\ ! mem (dom FRO.m{1}) x{1}); 1:by auto. 
   inline RRO.resample; exists* x{1}, r{1}; elim* => x1 r1.
@@ -444,7 +444,7 @@ abstract theory GenEager.
       (={x,y,FRO.m} /\ mem (dom FRO.m{1}) x{1} /\ (oget FRO.m{1}.[x{1}]).`2 = Unknown ==>
        ={x,y,FRO.m})
       (={x,y,FRO.m} /\ mem (dom FRO.m{1}) x{1} /\ (oget FRO.m{1}.[x{1}]).`2 = Unknown==>
-       ={x,y} /\ eq_except FRO.m{1} FRO.m{2} (fset1 x{1}) /\
+       ={x,y} /\ eq_except FRO.m{1} FRO.m{2} (pred1 x{1}) /\
        FRO.m{2}.[x{2}] = Some (y{2},Known)).
     + by move=> ? &mr [#] 2-> ? ? ?; exists FRO.m{mr}, y{mr}, x{mr}=> /#.
     + move=> ? &m &mr [#] <*> [#] 2-> Hex Hm2.
@@ -452,19 +452,19 @@ abstract theory GenEager.
     + symmetry; call (iter1_perm RRO.I iter_perm2); auto=> ? &mr [#] 3 -> Hdom Hm; split=> //=.
       by apply/perm_eq_sym/perm_to_rem/dom_restr; rewrite /in_dom_with Hdom.
     inline{1}Iter(RRO.I).iter_1s.
-    seq 3 1: (={x,y} /\ eq_except FRO.m{1} FRO.m{2} (fset1 x{1}) /\
+    seq 3 1: (={x,y} /\ eq_except FRO.m{1} FRO.m{2} (pred1 x{1}) /\
               l{1} = (elems (dom (restr Unknown FRO.m))){2} /\ !mem l{1} x{1} /\
               (FRO.m.[x]=Some(y, Known)){2}).
     + inline *; auto=> ? &mr [#] 3-> /= Hmem Hget; rewrite sampleto_ll=> ? _.
       by rewrite set2_eq_except getP_eq restr_set /= dom_rem -memE !inE negb_and.
     exists* x{1},y{1},(FRO.m.[x]{1}); elim* => x1 y1 mx1; pose mx2:= Some(y1,Known).
     call (iter_inv RRO.I (fun z=>x1<>z) 
-           (fun o1 o2 => eq_except o1 o2 (fset1 x1) /\ o1.[x1]= mx1 /\ o2.[x1]=mx2) 
+           (fun o1 o2 => eq_except o1 o2 (pred1 x1) /\ o1.[x1]= mx1 /\ o2.[x1]=mx2) 
            (I_f_eqex x1 mx1 mx2))=>/=.
     by auto=> ? &mr [#] -> <- 2-> ->> 2-> Hmem -> /#.
   exists* x{1},y{1},(FRO.m.[x]{1}); elim* => x1 y1 mx1; pose mx2:= Some(y1,Known).
   call (iter_inv RRO.I (fun z=>x1<>z) 
-         (fun o1 o2 => eq_except o1 o2 (fset1 x1) /\ o1.[x1]= mx1 /\ o2.[x1]=mx2) 
+         (fun o1 o2 => eq_except o1 o2 (pred1 x1) /\ o1.[x1]= mx1 /\ o2.[x1]=mx2) 
          (I_f_eqex x1 mx1 mx2))=> /=.
   auto=> ? &mr [#] -> <- 2-> ->> -> /= Hidm.
   rewrite restr_set getP_eq /mx2 eq_except_sym set_eq_except /=; split; [split|].
@@ -489,31 +489,31 @@ abstract theory GenEager.
     + symmetry; call (iter1_perm RRO.I iter_perm2); skip=> ? &mr [#] 2-> ? /=; split=> //.
       by apply/perm_eq_sym/perm_to_rem/dom_restr. 
     inline{1}Iter(RRO.I).iter_1s.
-    seq 3 1: (={x} /\ eq_except FRO.m{1} FRO.m{2} (fset1 x{1}) /\
+    seq 3 1: (={x} /\ eq_except FRO.m{1} FRO.m{2} (pred1 x{1}) /\
               l{1} = (elems (dom (restr Unknown FRO.m))){2} /\ !mem l{1} x{1} /\
               (FRO.m.[x]=None){2}).
     + inline *; auto=> ? ? [#] 2-> Hidm /=; rewrite sampleto_ll=> ? _.
-      rewrite eq_except_rem 1:!inE 2:set_eq_except // remP -memE in_fsetD1 negb_and /=.
+      rewrite eq_except_rem 2:set_eq_except // remP -memE in_fsetD1 negb_and /=.
       by rewrite restr_rem Hidm /= dom_rem.
     exists* x{1},(FRO.m.[x]{1}); elim* => x1 mx1.
     call (iter_inv RRO.I (fun z=>x1<>z) 
-           (fun o1 o2 => eq_except o1 o2 (fset1 x1) /\ o1.[x1]= mx1 /\ o2.[x1]=None) _).
+           (fun o1 o2 => eq_except o1 o2 (pred1 x1) /\ o1.[x1]= mx1 /\ o2.[x1]=None) _).
     + by conseq (I_f_eqex x1 mx1 None).
     auto=> ? &mr [#] 3-> ^Hex 2-> Hmem ^Hx -> /=.
     split=> [/#|_ mL mR [#] /eq_exceptP Hex' ? Heq].
     apply fmapP=> z; rewrite remP; case: (z=x{mr})=> [->/=|Hneq]; 1:by rewrite Heq.
-    by apply Hex'; rewrite inE.
+    by apply Hex'.
   inline RRO.resample; wp.
   exists *x{1},(FRO.m.[x]{1}); elim* => x1 mx1.
   call (iter_inv RRO.I (fun z=>x1<>z) 
-         (fun o1 o2 => eq_except o1 o2 (fset1 x1) /\ o1.[x1]= mx1 /\ o2.[x1]=None) _).
+         (fun o1 o2 => eq_except o1 o2 (pred1 x1) /\ o1.[x1]= mx1 /\ o2.[x1]=None) _).
   + by conseq (I_f_eqex x1 mx1 None).
   auto=> ? &mr [#] 4-> Hin /=.
-  rewrite restr_rem Hin /= remP eq_except_rem 1:inE // 1:eq_except_refl /=; split.
+  rewrite restr_rem Hin /= remP eq_except_rem // 1:eq_except_refl /=; split.
   + by move=> z; rewrite -memE dom_restr /#.
   move=> _ mL mR [#] /eq_exceptP Hex' ? Heq.
   apply fmapP=> z; rewrite remP; case: (z=x{mr})=> [->/=|Hneq]; 1:by rewrite Heq.
-  by apply Hex'; rewrite inE.
+  by apply Hex'.
   qed.
 
   lemma eager_in_dom:
@@ -523,8 +523,12 @@ abstract theory GenEager.
   eager proc; inline *; wp.
   while (={l,FRO.m} /\ (forall z, mem l z => in_dom_with FRO.m z Unknown){1} /\
          in_dom_with FRO.m{1} x{1} f{1} = result{2}).
-  + auto=> ? &mr [#] 2-> Hz <- ? _ /= ? -> /=.
-    by split=> [z /mem_drop Hm|]; rewrite /in_dom_with dom_set getP !inE /#.
+  + auto=> &m1 &m2 [#] 2-> Hz <- ? _ /= ? -> /=.
+    split=> [z /mem_drop Hm|]; rewrite /in_dom_with dom_set getP !inE.
+      smt ().
+    case: (x{m1} = head witness l{m2})=> //=.
+    rewrite oget_some /=; have + ->>:= Hz (head witness l{m2}) _; 1: smt.
+    by rewrite /in_dom_with=>- [] -> ->.    
   by auto=> ? &mr /= [#] 3-> /=; split=> // z; rewrite -memE dom_restr.
   qed.
 
@@ -559,7 +563,7 @@ abstract theory GenEager.
       by apply/perm_eq_sym/perm_to_rem; rewrite restr_set /= dom_set !inE.
     + by move=> ? &mr [#] 2-> ?; exists FRO.m{mr}, x{mr}.
     inline Iter(RRO.I).iter_1s RRO.I.f RRO.resample; wp; swap{1} -1.
-    seq  1  7: (={x} /\ eq_except FRO.m{1} FRO.m{2} (fset1 x{1}) /\
+    seq  1  7: (={x} /\ eq_except FRO.m{1} FRO.m{2} (pred1 x{1}) /\
                 l{2} = (elems (dom (restr Unknown FRO.m))){1} /\
                 (FRO.m.[x]){2} = Some(c{1},Unknown) /\ (FRO.m.[x]){1} = None).
     + wp; rnd; auto=> ? &mr [#] 2->; rewrite in_dom sampleto_ll /= => Heq ? _ ? ->.
@@ -567,7 +571,7 @@ abstract theory GenEager.
       congr; apply fsetP=> z; rewrite in_fsetD1 dom_restr /in_dom_with !in_dom /#.
     exists* x{1},c{1}; elim* => x1 c1; pose mx2:= Some(c1,Unknown).
     call (iter_inv RRO.I (fun z=>x1<>z) 
-           (fun o1 o2 => eq_except o1 o2 (fset1 x1) /\ o1.[x1]= None /\ o2.[x1]=mx2) _).
+           (fun o1 o2 => eq_except o1 o2 (pred1 x1) /\ o1.[x1]= None /\ o2.[x1]=mx2) _).
     + by conseq (I_f_eqex x1 None mx2).
     auto=> ? &mr [#] 2<- -> ^Hex 3-> ^Hx1 -> @/mx2 /=; split=> [z|_ mL mR [#]].
     + by rewrite -memE dom_restr /in_dom_with in_dom /#.
